progress in implementing LinkedBetree. BufferStack no longer contains BufferDiskView. The BufferDiskView is held solely by the LinkedBetree node. The LinkedBetree provides the disk contexts for interpreting both the BetreeNode and BufferStack datatypes

Splinter/Betree/FilteredBetree.i.dfy
@@ -6,6 +6,7 @@ include "../../lib/Base/total_order.i.dfy"
 include "../../lib/Buckets/BoundedPivotsLib.i.dfy"
 include "Domain.i.dfy"
 include "SplitRequest.i.dfy"
+include "BufferOffsets.i.dfy"
 
 // In contrast to the PivotBetree above, upon flushing a buffer down the tree, 
 // the FilteredBetree keeps the entire buffer but notes that it should filter out the keys in 
@@ -29,6 +30,7 @@ module FilteredBetree
   import opened BoundedPivotsLib
   import opened DomainMod
   import opened SplitRequestMod
+  import opened BufferOffsetsMod
 
   datatype TransitionLabel =
     QueryLabel(endLsn: LSN, key: Key, value: Value)
@@ -38,81 +40,6 @@ module FilteredBetree
   | InternalLabel()
 
   type Element = Upperbounded_Lexicographic_Byte_Order_Impl.Ord.Element
-
-  // data structure tracking offsets of buffers
-  datatype BufferOffsets = BufferOffsets(offsets: seq<nat>)
-  {
-    function Size() : nat
-    {
-      |offsets|
-    }
-
-    function Get(i: nat) : nat
-      requires i < |offsets|
-    {
-      offsets[i]
-    }
-
-    function Slice(start: nat, end: nat) : (out: BufferOffsets)
-      requires start <= end <= |offsets|
-      ensures out.Size() == end-start
-      ensures forall i:nat | i < out.Size() :: out.Get(i) == Get(i+start)
-    {
-      BufferOffsets(offsets[start..end])
-    }
-
-    predicate CanCollectGarbage(count: nat)
-    {
-      forall i:nat | i < Size() :: count <= Get(i)
-    }
-
-    // # to shift for every child
-    function CollectGarbage(count: nat) : (out: BufferOffsets)
-      requires CanCollectGarbage(count)
-    {
-      BufferOffsets(seq (Size(), i requires 0 <= i < Size() => Get(i)-count))
-    }
-
-    function AdvanceIndex(idx: nat, newOffset: nat) : (out: BufferOffsets)
-      requires idx < Size()
-      ensures out.Size() == Size()
-      ensures forall i: nat | i < Size() && i != idx :: Get(i) == out.Get(i)
-    {
-      BufferOffsets(offsets[idx := newOffset])
-    }
-
-    // shift the value of each entry based on compacted buffers
-    function CompactRange(compactStart: nat, compactEnd: nat, bufferLen: nat) : (out: BufferOffsets)
-      requires compactStart < compactEnd <= bufferLen
-      ensures forall offset | offset in out.offsets :: offset <= bufferLen
-      ensures out.Size() == Size()
-      ensures forall offset | offset in out.offsets :: offset  <= bufferLen - (compactEnd-compactStart-1)
-    {
-      CompactInternal(compactStart, compactEnd, bufferLen, Size())
-    }
-
-    function CompactInternal(compactStart: nat, compactEnd: nat, bufferLen: nat, count: nat) : (out: BufferOffsets)
-      requires compactStart < compactEnd <= bufferLen
-      requires forall i:nat | i < Size() :: Get(i) <= bufferLen
-      requires count <= Size()
-      ensures out.Size() == count
-      ensures (forall offset | offset in out.offsets :: offset <= bufferLen - (compactEnd-compactStart-1))
-    {
-      if count == 0 then BufferOffsets([])
-      else (
-        var numFlushed := Get(count-1); // this many buffers have been flushed
-        var end := bufferLen-numFlushed; // end of valid active buffers 
-        var numFlushed' := 
-          if compactStart >= end // compacted range is entirely in flushed range
-          then numFlushed - (compactEnd-compactStart-1)
-          else if compactEnd <= end // compacted range is entirely outside the flushed range
-          then numFlushed
-          else numFlushed - (compactEnd - end); // compacted range overlaps with flushed range
-
-        BufferOffsets(CompactInternal(compactStart, compactEnd, bufferLen, count-1).offsets + [numFlushed'])
-      )
-    }
-  }
 
   predicate WFChildren(children: seq<BetreeNode>)
   {
@@ -134,7 +61,7 @@ module FilteredBetree
           && WFPivots(pivotTable)
           && |children| == NumBuckets(pivotTable)
           && |children| == flushedOffsets.Size()
-          && (forall ofs | ofs in flushedOffsets.offsets :: ofs <= buffers.Length())
+          && flushedOffsets.BoundedBy(buffers.Length())
         )
     }
 
@@ -258,10 +185,7 @@ module FilteredBetree
       var oldChild := children[request.childIdx];
       var (newLeftChild, newRightChild) := if request.SplitLeaf? then oldChild.SplitLeaf(request.splitKey) else oldChild.SplitIndex(request.childPivotIdx);
       var newChildren := replace1with2(children, newLeftChild, newRightChild, request.childIdx);
-
-      var childFlushedBuffer := flushedOffsets.Get(request.childIdx);
-      var newflushedOffsets := BufferOffsets(replace1with2(flushedOffsets.offsets, childFlushedBuffer, childFlushedBuffer, request.childIdx));
-
+      var newflushedOffsets := flushedOffsets.Split(request.childIdx);
       BetreeNode(buffers, InsertPivot(pivotTable, request.childIdx+1, SplitKey(request)), newChildren, newflushedOffsets)
     }
 
