Splinter/Betree/BufferOffsets.i.dfy
@@ -1,0 +1,97 @@
+// Copyright 2018-2021 VMware, Inc., Microsoft Inc., Carnegie Mellon University, ETH Zurich, and University of Washington
+// SPDX-License-Identifier: BSD-2-Clause
+
+include "../../lib/Base/Sequences.i.dfy"
+
+module BufferOffsetsMod
+{
+  import opened Sequences
+
+// data structure tracking offsets of buffers
+  datatype BufferOffsets = BufferOffsets(offsets: seq<nat>)
+  {
+    function Size() : nat
+    {
+      |offsets|
+    }
+
+    function Get(i: nat) : nat
+      requires i < |offsets|
+    {
+      offsets[i]
+    }
+
+    predicate BoundedBy(length: nat) {
+      forall ofs | ofs in offsets :: ofs <= length
+    }
+
+    function Slice(start: nat, end: nat) : (out: BufferOffsets)
+      requires start <= end <= |offsets|
+      ensures out.Size() == end-start
+      ensures forall i:nat | i < out.Size() :: out.Get(i) == Get(i+start)
+    {
+      BufferOffsets(offsets[start..end])
+    }
+
+    function Split(idx: nat) : (out: BufferOffsets) 
+      requires idx < |offsets|
+    {
+      var original := Get(idx);
+      BufferOffsets(replace1with2(offsets, original, original, idx))
+    }
+
+    predicate CanCollectGarbage(count: nat)
+    {
+      forall i:nat | i < Size() :: count <= Get(i)
+    }
+
+    // # to shift for every child
+    function CollectGarbage(count: nat) : (out: BufferOffsets)
+      requires CanCollectGarbage(count)
+    {
+      BufferOffsets(seq (Size(), i requires 0 <= i < Size() => Get(i)-count))
+    }
+
+    function AdvanceIndex(idx: nat, newOffset: nat) : (out: BufferOffsets)
+      requires idx < Size()
+      ensures out.Size() == Size()
+      ensures forall i: nat | i < Size() && i != idx :: Get(i) == out.Get(i)
+    {
+      BufferOffsets(offsets[idx := newOffset])
+    }
+
+    // shift the value of each entry based on compacted buffers
+    function CompactRange(compactStart: nat, compactEnd: nat, bufferLen: nat) : (out: BufferOffsets)
+      requires compactStart < compactEnd <= bufferLen
+      requires BoundedBy(bufferLen)
+      ensures forall offset | offset in out.offsets :: offset <= bufferLen
+      ensures out.Size() == Size()
+      ensures forall offset | offset in out.offsets :: offset  <= bufferLen - (compactEnd-compactStart-1)
+    {
+      CompactInternal(compactStart, compactEnd, bufferLen, Size())
+    }
+
+    function CompactInternal(compactStart: nat, compactEnd: nat, bufferLen: nat, count: nat) : (out: BufferOffsets)
+      requires compactStart < compactEnd <= bufferLen
+      requires BoundedBy(bufferLen)
+      requires count <= Size()
+      ensures out.Size() == count
+      ensures out.BoundedBy(bufferLen - (compactEnd-compactStart-1))
+    {
+    
+      if count == 0 then BufferOffsets([])
+      else (
+        var numFlushed := Get(count-1); // this many buffers have been flushed
+        var end := bufferLen-numFlushed; // end of valid active buffers 
+        var numFlushed' := 
+          if compactStart >= end // compacted range is entirely in flushed range
+          then numFlushed - (compactEnd-compactStart-1)
+          else if compactEnd <= end // compacted range is entirely outside the flushed range
+          then numFlushed
+          else numFlushed - (compactEnd - end); // compacted range overlaps with flushed range
+
+        BufferOffsets(CompactInternal(compactStart, compactEnd, bufferLen, count-1).offsets + [numFlushed'])
+      )
+    }
+  }
+}
